hax-lib/proof-libs/lean/Hax/rust_primitives/ops.lean
@@ -1,6 +1,7 @@
-import Hax.rust_primitives.USize64
 import Hax.Tactic.Init
+import Hax.rust_primitives.USize64
 import Hax.Tactic.SpecSet
+import Hax.MissingLean
 import Hax.rust_primitives.RustM
 open Std.Do
 open Std.Tactic
@@ -15,13 +16,13 @@ abbrev u8 := UInt8
 abbrev u16 := UInt16
 abbrev u32 := UInt32
 abbrev u64 := UInt64
+abbrev u128 := UInt128
 abbrev usize := USize64
-abbrev u128 := BitVec 128
 abbrev i8 := Int8
 abbrev i16 := Int16
 abbrev i32 := Int32
 abbrev i64 := Int64
-abbrev i128 := BitVec 128
+abbrev i128 := Int128
 abbrev isize := ISize
 
 abbrev f32 := Float32
@@ -35,6 +36,9 @@ attribute [grind] ToNat.toNat
 
 @[simp, grind]
 instance : ToNat usize where
+  toNat x := x.toNat
+@[simp, grind]
+instance : ToNat u128 where
   toNat x := x.toNat
 @[simp, grind]
 instance : ToNat u64 where
@@ -175,11 +179,13 @@ declare_Hax_int_ops unsigned UInt8 8
 declare_Hax_int_ops unsigned UInt16 16
 declare_Hax_int_ops unsigned UInt32 32
 declare_Hax_int_ops unsigned UInt64 64
+declare_Hax_int_ops unsigned UInt128 128
 declare_Hax_int_ops unsigned USize64 64
 declare_Hax_int_ops signed Int8 8
 declare_Hax_int_ops signed Int16 16
 declare_Hax_int_ops signed Int32 32
 declare_Hax_int_ops signed Int64 64
+declare_Hax_int_ops signed Int128 128
 declare_Hax_int_ops signed ISize System.Platform.numBits
 
 
@@ -193,11 +199,13 @@ macro "declare_Hax_shift_ops" : command => do
     ("UInt16", ← `(term| 16)),
     ("UInt32", ← `(term| 32)),
     ("UInt64", ← `(term| 64)),
+    ("UInt128", ← `(term| 128)),
     ("USize64", ← `(term| 64)),
     ("Int8", ← `(term| 8)),
     ("Int16", ← `(term| 16)),
     ("Int32", ← `(term| 32)),
     ("Int64", ← `(term| 64)),
+    ("Int128", ← `(term| 128)),
     ("ISize", ← `(term| OfNat.ofNat System.Platform.numBits))
   ]
   for (ty1, width1) in tys do
@@ -328,11 +336,13 @@ declare_Hax_int_ops_spec unsigned UInt8 8
 declare_Hax_int_ops_spec unsigned UInt16 16
 declare_Hax_int_ops_spec unsigned UInt32 32
 declare_Hax_int_ops_spec unsigned UInt64 64
+declare_Hax_int_ops_spec unsigned UInt128 128
 declare_Hax_int_ops_spec unsigned USize64 64
 declare_Hax_int_ops_spec signed Int8 8
 declare_Hax_int_ops_spec signed Int16 16
 declare_Hax_int_ops_spec signed Int32 32
 declare_Hax_int_ops_spec signed Int64 64
+declare_Hax_int_ops_spec signed Int128 128
 declare_Hax_int_ops_spec signed ISize System.Platform.numBits
 
 open Lean in
@@ -343,10 +353,12 @@ macro "declare_Hax_shift_ops_spec" : command => do
     ("UInt16", ← `(term| 16)),
     ("UInt32", ← `(term| 32)),
     ("UInt64", ← `(term| 64)),
+    ("UInt128", ← `(term| 128)),
     ("Int8", ← `(term| 8)),
     ("Int16", ← `(term| 16)),
     ("Int32", ← `(term| 32)),
     ("Int64", ← `(term| 64)),
+    ("Int128", ← `(term| 128)),
   ]
   for (ty1, width1) in tys do
     for (ty2, _width2) in tys do
